<?xml version="1.0"?>
<rdf:RDF xmlns="http://www.semanticweb.org/djebbia/ontologies/2022/8/untitled-ontology-22/"
     xml:base="http://www.semanticweb.org/djebbia/ontologies/2022/8/untitled-ontology-22/"
     xmlns:owl="http://www.w3.org/2002/07/owl#"
     xmlns:rdf="http://www.w3.org/1999/02/22-rdf-syntax-ns#"
     xmlns:xml="http://www.w3.org/XML/1998/namespace"
     xmlns:xsd="http://www.w3.org/2001/XMLSchema#"
     xmlns:rdfs="http://www.w3.org/2000/01/rdf-schema#">
    <owl:Ontology rdf:about="http://www.semanticweb.org/djebbia/ontologies/2022/8/untitled-ontology-22"/>
    


    <!-- 
    ///////////////////////////////////////////////////////////////////////////////////////
    //
    // Classes
    //
    ///////////////////////////////////////////////////////////////////////////////////////
     -->

    


    <!-- http://purl.org/dc/elements/1.1/bibliographicCitation -->

    <owl:Class rdf:about="http://purl.org/dc/elements/1.1/bibliographicCitation">
        <rdfs:subClassOf rdf:resource="http://www.semanticweb.org/djebbia/ontologies/2022/8/untitled-ontology-22/multimedia_extended_metadata"/>
        <rdfs:comment xml:lang="en">CC BY-SA</rdfs:comment>
        <rdfs:comment xml:lang="en">dc:bibliographicCitation</rdfs:comment>
        <rdfs:comment rdf:datatype="http://www.w3.org/2001/XMLSchema#anyURI">http://creativecommons.org/licenses/by-sa/4.0/</rdfs:comment>
        <rdfs:isDefinedBy rdf:datatype="http://www.w3.org/2001/XMLSchema#anyURI">http://purl.org/dc/terms/bibliographicCitation</rdfs:isDefinedBy>
        <rdfs:label xml:lang="en">dc:bibliographicCitation</rdfs:label>
    </owl:Class>
    


    <!-- http://www.semanticweb.org/djebbia/ontologies/2022/8/untitled-ontology-22/BrightnessValue -->

    <owl:Class rdf:about="http://www.semanticweb.org/djebbia/ontologies/2022/8/untitled-ontology-22/BrightnessValue">
        <rdfs:subClassOf rdf:resource="http://www.semanticweb.org/djebbia/ontologies/2022/8/untitled-ontology-22/multimedia_extended_metadata"/>
        <rdfs:comment xml:lang="en">CC BY-SA</rdfs:comment>
        <rdfs:comment xml:lang="en">EXIF tag 37379, 0x9203. Brightness, unit is APEX.</rdfs:comment>
        <rdfs:comment xml:lang="en">exif:BrightnessValue</rdfs:comment>
        <rdfs:comment rdf:datatype="http://www.w3.org/2001/XMLSchema#anyURI">http://creativecommons.org/licenses/by-sa/4.0/</rdfs:comment>
        <rdfs:isDefinedBy rdf:datatype="http://www.w3.org/2001/XMLSchema#anyURI">https://developer.adobe.com/xmp/docs/XMPNamespaces/exif/</rdfs:isDefinedBy>
        <rdfs:label xml:lang="en">BrightnessValue</rdfs:label>
    </owl:Class>
    


    <!-- http://www.semanticweb.org/djebbia/ontologies/2022/8/untitled-ontology-22/DerivedFrom -->

    <owl:Class rdf:about="http://www.semanticweb.org/djebbia/ontologies/2022/8/untitled-ontology-22/DerivedFrom">
        <rdfs:subClassOf rdf:resource="http://www.semanticweb.org/djebbia/ontologies/2022/8/untitled-ontology-22/Multimedia"/>
        <rdfs:comment xml:lang="en">CC BY-SA</rdfs:comment>
        <rdfs:comment xml:lang="en">eference to the original document from which this one is derived. It is a minimal reference; missing components can be assumed to be unchanged. For example, a new version might only need to specify the instance ID and version number of the previous version, or a rendition might only need to specify the instance ID and rendition class of the original.</rdfs:comment>
        <rdfs:comment rdf:datatype="http://www.w3.org/2001/XMLSchema#anyURI">http://creativecommons.org/licenses/by-sa/4.0/</rdfs:comment>
        <rdfs:comment xml:lang="en">xmpMM:DerivedFrom</rdfs:comment>
        <rdfs:isDefinedBy rdf:datatype="http://www.w3.org/2001/XMLSchema#anyURI">https://developer.adobe.com/xmp/docs/XMPNamespaces/xmpMM/</rdfs:isDefinedBy>
        <rdfs:label xml:lang="en">DerivedFrom</rdfs:label>
    </owl:Class>
    


    <!-- http://www.semanticweb.org/djebbia/ontologies/2022/8/untitled-ontology-22/EXIF -->

    <owl:Class rdf:about="http://www.semanticweb.org/djebbia/ontologies/2022/8/untitled-ontology-22/EXIF">
        <rdfs:subClassOf rdf:resource="http://www.semanticweb.org/djebbia/ontologies/2022/8/untitled-ontology-22/standards"/>
        <rdfs:comment xml:lang="en">CC BY-SA</rdfs:comment>
        <rdfs:comment xml:lang="en">The date and time the resource was last modified. NOTE: The value of this property is not necessarily the same as the file’s system modification date because it is typically set before the file is saved.</rdfs:comment>
        <rdfs:comment rdf:datatype="http://www.w3.org/2001/XMLSchema#anyURI">http://creativecommons.org/licenses/by-sa/4.0/</rdfs:comment>
        <rdfs:label xml:lang="en">EXIF</rdfs:label>
    </owl:Class>
    


    <!-- http://www.semanticweb.org/djebbia/ontologies/2022/8/untitled-ontology-22/EXIV2 -->

    <owl:Class rdf:about="http://www.semanticweb.org/djebbia/ontologies/2022/8/untitled-ontology-22/EXIV2">
        <rdfs:subClassOf rdf:resource="http://www.semanticweb.org/djebbia/ontologies/2022/8/untitled-ontology-22/standards"/>
        <rdfs:comment xml:lang="en">CC BY-SA</rdfs:comment>
        <rdfs:comment xml:lang="en">The date and time the resource was last modified. NOTE: The value of this property is not necessarily the same as the file’s system modification date because it is typically set before the file is saved.</rdfs:comment>
        <rdfs:comment rdf:datatype="http://www.w3.org/2001/XMLSchema#anyURI">http://creativecommons.org/licenses/by-sa/4.0/</rdfs:comment>
        <rdfs:label xml:lang="en">EXIV2</rdfs:label>
    </owl:Class>
    


    <!-- http://www.semanticweb.org/djebbia/ontologies/2022/8/untitled-ontology-22/IQ_metadata -->

    <owl:Class rdf:about="http://www.semanticweb.org/djebbia/ontologies/2022/8/untitled-ontology-22/IQ_metadata"/>
    


    <!-- http://www.semanticweb.org/djebbia/ontologies/2022/8/untitled-ontology-22/ListOfMetadataStandards -->

    <owl:Class rdf:about="http://www.semanticweb.org/djebbia/ontologies/2022/8/untitled-ontology-22/ListOfMetadataStandards">
        <rdfs:subClassOf rdf:resource="http://www.semanticweb.org/djebbia/ontologies/2022/8/untitled-ontology-22/standards"/>
        <rdfs:comment xml:lang="en">CC BY-SA</rdfs:comment>
        <rdfs:comment xml:lang="en">The date and time the resource was last modified. NOTE: The value of this property is not necessarily the same as the file’s system modification date because it is typically set before the file is saved.</rdfs:comment>
        <rdfs:comment rdf:datatype="http://www.w3.org/2001/XMLSchema#anyURI">http://creativecommons.org/licenses/by-sa/4.0/</rdfs:comment>
        <rdfs:label xml:lang="en">List of Metadata Standards</rdfs:label>
    </owl:Class>
    


    <!-- http://www.semanticweb.org/djebbia/ontologies/2022/8/untitled-ontology-22/Multimedia -->

    <owl:Class rdf:about="http://www.semanticweb.org/djebbia/ontologies/2022/8/untitled-ontology-22/Multimedia"/>
    


    <!-- http://www.semanticweb.org/djebbia/ontologies/2022/8/untitled-ontology-22/PLUS -->

    <owl:Class rdf:about="http://www.semanticweb.org/djebbia/ontologies/2022/8/untitled-ontology-22/PLUS">
        <rdfs:subClassOf rdf:resource="http://www.semanticweb.org/djebbia/ontologies/2022/8/untitled-ontology-22/standards"/>
        <rdfs:comment xml:lang="en">CC BY-SA</rdfs:comment>
        <rdfs:comment xml:lang="en">The date and time the resource was last modified. NOTE: The value of this property is not necessarily the same as the file’s system modification date because it is typically set before the file is saved.</rdfs:comment>
        <rdfs:comment rdf:datatype="http://www.w3.org/2001/XMLSchema#anyURI">http://creativecommons.org/licenses/by-sa/4.0/</rdfs:comment>
        <rdfs:label xml:lang="en">PLUS</rdfs:label>
    </owl:Class>
    


    <!-- http://www.semanticweb.org/djebbia/ontologies/2022/8/untitled-ontology-22/SubjectCode -->

    <owl:Class rdf:about="http://www.semanticweb.org/djebbia/ontologies/2022/8/untitled-ontology-22/SubjectCode">
        <rdfs:subClassOf rdf:resource="http://www.semanticweb.org/djebbia/ontologies/2022/8/untitled-ontology-22/Multimedia"/>
        <rdfs:comment xml:lang="en">CC BY-SA</rdfs:comment>
        <rdfs:comment xml:lang="en">Iptc4xmpCore:SubjectCode</rdfs:comment>
        <rdfs:comment rdf:datatype="http://www.w3.org/2001/XMLSchema#anyURI">http://creativecommons.org/licenses/by-sa/4.0/</rdfs:comment>
        <rdfs:comment xml:lang="en">pecifies one or more Subjects from the IPTC Subject-NewsCodes taxonomy to categorise the image. Each Subject is represented as a string of 8 digits in an unordered list.</rdfs:comment>
        <rdfs:isDefinedBy rdf:datatype="http://www.w3.org/2001/XMLSchema#anyURI">https://www.iptc.org/std/photometadata/specification/IPTC-PhotoMetadata-2021.1.html#subject-code</rdfs:isDefinedBy>
        <rdfs:label xml:lang="en">SubjectCode</rdfs:label>
    </owl:Class>
    


    <!-- http://www.semanticweb.org/djebbia/ontologies/2022/8/untitled-ontology-22/TDWGSpecimenLSIDOntology -->

    <owl:Class rdf:about="http://www.semanticweb.org/djebbia/ontologies/2022/8/untitled-ontology-22/TDWGSpecimenLSIDOntology">
        <rdfs:subClassOf rdf:resource="http://www.semanticweb.org/djebbia/ontologies/2022/8/untitled-ontology-22/standards"/>
        <rdfs:comment xml:lang="en">CC BY-SA</rdfs:comment>
        <rdfs:comment xml:lang="en">The date and time the resource was last modified. NOTE: The value of this property is not necessarily the same as the file’s system modification date because it is typically set before the file is saved.</rdfs:comment>
        <rdfs:comment rdf:datatype="http://www.w3.org/2001/XMLSchema#anyURI">http://creativecommons.org/licenses/by-sa/4.0/</rdfs:comment>
        <rdfs:label xml:lang="en">TDWG Specimen LSID Ontology</rdfs:label>
    </owl:Class>
    


    <!-- http://www.semanticweb.org/djebbia/ontologies/2022/8/untitled-ontology-22/TransmissionReference -->

    <owl:Class rdf:about="http://www.semanticweb.org/djebbia/ontologies/2022/8/untitled-ontology-22/TransmissionReference">
        <rdfs:subClassOf rdf:resource="http://www.semanticweb.org/djebbia/ontologies/2022/8/untitled-ontology-22/Multimedia"/>
        <rdfs:comment xml:lang="en">CC BY-SA</rdfs:comment>
        <rdfs:comment xml:lang="en">Number or identifier for the purpose of improved workflow handling. This is a user created identifier related to the job for which the image is supplied.</rdfs:comment>
        <rdfs:comment rdf:datatype="http://www.w3.org/2001/XMLSchema#anyURI">http://creativecommons.org/licenses/by-sa/4.0/</rdfs:comment>
        <rdfs:comment xml:lang="en">photoshop:TransmissionReference </rdfs:comment>
        <rdfs:isDefinedBy rdf:datatype="http://www.w3.org/2001/XMLSchema#anyURI">https://www.iptc.org/std/photometadata/specification/IPTC-PhotoMetadata-2021.1.html#job-id</rdfs:isDefinedBy>
        <rdfs:label xml:lang="en">TransmissionReference</rdfs:label>
    </owl:Class>
    


    <!-- http://www.semanticweb.org/djebbia/ontologies/2022/8/untitled-ontology-22/XMP -->

    <owl:Class rdf:about="http://www.semanticweb.org/djebbia/ontologies/2022/8/untitled-ontology-22/XMP">
        <rdfs:subClassOf rdf:resource="http://www.semanticweb.org/djebbia/ontologies/2022/8/untitled-ontology-22/standards"/>
        <rdfs:comment xml:lang="en">CC BY-SA</rdfs:comment>
        <rdfs:comment xml:lang="en">The date and time the resource was last modified. NOTE: The value of this property is not necessarily the same as the file’s system modification date because it is typically set before the file is saved.</rdfs:comment>
        <rdfs:comment rdf:datatype="http://www.w3.org/2001/XMLSchema#anyURI">http://creativecommons.org/licenses/by-sa/4.0/</rdfs:comment>
        <rdfs:isDefinedBy rdf:datatype="http://www.w3.org/2001/XMLSchema#anyURI">https://archimedespalimpsest.net/Documents/External/XMP/</rdfs:isDefinedBy>
        <rdfs:label xml:lang="en">XMP</rdfs:label>
        <rdfs:label xml:lang="en">XMP </rdfs:label>
    </owl:Class>
    


    <!-- http://www.semanticweb.org/djebbia/ontologies/2022/8/untitled-ontology-22/XMPMediaManagement -->

    <owl:Class rdf:about="http://www.semanticweb.org/djebbia/ontologies/2022/8/untitled-ontology-22/XMPMediaManagement">
        <rdfs:subClassOf rdf:resource="http://www.semanticweb.org/djebbia/ontologies/2022/8/untitled-ontology-22/standards"/>
        <rdfs:comment xml:lang="en">CC BY-SA</rdfs:comment>
        <rdfs:comment xml:lang="en">The date and time the resource was last modified. NOTE: The value of this property is not necessarily the same as the file’s system modification date because it is typically set before the file is saved.</rdfs:comment>
        <rdfs:comment rdf:datatype="http://www.w3.org/2001/XMLSchema#anyURI">http://creativecommons.org/licenses/by-sa/4.0/</rdfs:comment>
        <rdfs:label xml:lang="en">XMPMediaManagement </rdfs:label>
    </owl:Class>
    


    <!-- http://www.semanticweb.org/djebbia/ontologies/2022/8/untitled-ontology-22/accessRights -->

    <owl:Class rdf:about="http://www.semanticweb.org/djebbia/ontologies/2022/8/untitled-ontology-22/accessRights">
        <rdfs:subClassOf rdf:resource="http://www.semanticweb.org/djebbia/ontologies/2022/8/untitled-ontology-22/Multimedia"/>
        <rdfs:comment xml:lang="en">CC BY-SA</rdfs:comment>
        <rdfs:comment xml:lang="en">Information about who can access the resource or an indication of its security</rdfs:comment>
        <rdfs:comment xml:lang="en">dcterms:accessRights</rdfs:comment>
        <rdfs:comment rdf:datatype="http://www.w3.org/2001/XMLSchema#anyURI">http://creativecommons.org/licenses/by-sa/4.0/</rdfs:comment>
        <rdfs:isDefinedBy rdf:datatype="http://www.w3.org/2001/XMLSchema#anyURI">http://purl.org/dc/terms/accessRights</rdfs:isDefinedBy>
        <rdfs:label xml:lang="en">accessRights</rdfs:label>
    </owl:Class>
    


    <!-- http://www.semanticweb.org/djebbia/ontologies/2022/8/untitled-ontology-22/arc_id -->

    <owl:Class rdf:about="http://www.semanticweb.org/djebbia/ontologies/2022/8/untitled-ontology-22/arc_id">
        <rdfs:subClassOf rdf:resource="http://www.semanticweb.org/djebbia/ontologies/2022/8/untitled-ontology-22/IQ_metadata"/>
        <rdfs:subClassOf rdf:resource="http://www.semanticweb.org/djebbia/ontologies/2022/8/untitled-ontology-22/Multimedia"/>
        <rdfs:subClassOf rdf:resource="http://www.semanticweb.org/djebbia/ontologies/2022/8/untitled-ontology-22/multimedia_extended_metadata"/>
        <rdfs:comment xml:lang="en">A unqiue idientifier for each inviidual image.</rdfs:comment>
        <rdfs:comment xml:lang="en">An unambiguous reference to the resource within a given context.</rdfs:comment>
        <rdfs:comment xml:lang="en">CC BY-SA</rdfs:comment>
        <rdfs:comment xml:lang="en">dc:identifier</rdfs:comment>
        <rdfs:comment rdf:datatype="http://www.w3.org/2001/XMLSchema#anyURI">http://creativecommons.org/licenses/by-sa/4.0/</rdfs:comment>
        <rdfs:isDefinedBy rdf:datatype="http://www.w3.org/2001/XMLSchema#anyURI">http://purl.org/dc/terms/identifier</rdfs:isDefinedBy>
        <rdfs:label xml:lang="en">arc_id</rdfs:label>
    </owl:Class>
    


    <!-- http://www.semanticweb.org/djebbia/ontologies/2022/8/untitled-ontology-22/associatedMedia -->

    <owl:Class rdf:about="http://www.semanticweb.org/djebbia/ontologies/2022/8/untitled-ontology-22/associatedMedia">
        <rdfs:subClassOf rdf:resource="http://www.semanticweb.org/djebbia/ontologies/2022/8/untitled-ontology-22/Multimedia"/>
        <rdfs:comment xml:lang="en">A list (concatenated and separated) of identifiers (publication, global unique identifier, URI) of media associated with the Occurrence.</rdfs:comment>
        <rdfs:comment xml:lang="en">CC BY-SA</rdfs:comment>
        <rdfs:comment xml:lang="en">dwc:associatedMedia</rdfs:comment>
        <rdfs:comment rdf:datatype="http://www.w3.org/2001/XMLSchema#anyURI">http://creativecommons.org/licenses/by-sa/4.0/</rdfs:comment>
        <rdfs:isDefinedBy rdf:datatype="http://www.w3.org/2001/XMLSchema#anyURI">http://rs.tdwg.org/dwc/terms/associatedMedia</rdfs:isDefinedBy>
        <rdfs:label xml:lang="en">associatedMedia</rdfs:label>
    </owl:Class>
    


    <!-- http://www.semanticweb.org/djebbia/ontologies/2022/8/untitled-ontology-22/audobonCore -->

    <owl:Class rdf:about="http://www.semanticweb.org/djebbia/ontologies/2022/8/untitled-ontology-22/audobonCore">
        <rdfs:subClassOf rdf:resource="http://www.semanticweb.org/djebbia/ontologies/2022/8/untitled-ontology-22/standards"/>
        <rdfs:comment xml:lang="en">CC BY-SA</rdfs:comment>
        <rdfs:comment xml:lang="en">The date and time the resource was last modified. NOTE: The value of this property is not necessarily the same as the file’s system modification date because it is typically set before the file is saved.</rdfs:comment>
        <rdfs:comment rdf:datatype="http://www.w3.org/2001/XMLSchema#anyURI">http://creativecommons.org/licenses/by-sa/4.0/</rdfs:comment>
        <rdfs:label xml:lang="en">audobonCore</rdfs:label>
    </owl:Class>
    


    <!-- http://www.semanticweb.org/djebbia/ontologies/2022/8/untitled-ontology-22/batch_id -->

    <owl:Class rdf:about="http://www.semanticweb.org/djebbia/ontologies/2022/8/untitled-ontology-22/batch_id">
        <rdfs:subClassOf rdf:resource="http://www.semanticweb.org/djebbia/ontologies/2022/8/untitled-ontology-22/Multimedia"/>
        <rdfs:comment xml:lang="en">CC BY-SA</rdfs:comment>
        <rdfs:comment xml:lang="en">References an external job management file for a job process in which the document is being used. Use of job names is under user control. Typical use would be to identify all documents that are part of a particular job or contract. There are multiple values because there can be more than one job using a particular document at any time, and it can also be useful to keep historical information about what jobs a document was part of previously.</rdfs:comment>
        <rdfs:comment rdf:datatype="http://www.w3.org/2001/XMLSchema#anyURI">http://creativecommons.org/licenses/by-sa/4.0/</rdfs:comment>
        <rdfs:comment xml:lang="en">xmpBJ:JobRef</rdfs:comment>
        <rdfs:isDefinedBy rdf:datatype="http://www.w3.org/2001/XMLSchema#anyURI">https://developer.adobe.com/xmp/docs/XMPNamespaces/xmpBJ/</rdfs:isDefinedBy>
        <rdfs:label xml:lang="en">batch_id</rdfs:label>
    </owl:Class>
    


    <!-- http://www.semanticweb.org/djebbia/ontologies/2022/8/untitled-ontology-22/brightness -->

    <owl:Class rdf:about="http://www.semanticweb.org/djebbia/ontologies/2022/8/untitled-ontology-22/brightness">
        <rdfs:subClassOf rdf:resource="http://www.semanticweb.org/djebbia/ontologies/2022/8/untitled-ontology-22/multimedia_extended_metadata"/>
        <rdfs:comment xml:lang="en">Brightness setting. Range 0 to 150</rdfs:comment>
        <rdfs:comment xml:lang="en">CC BY-SA</rdfs:comment>
        <rdfs:comment xml:lang="en">crs:Brightness</rdfs:comment>
        <rdfs:comment rdf:datatype="http://www.w3.org/2001/XMLSchema#anyURI">http://creativecommons.org/licenses/by-sa/4.0/</rdfs:comment>
        <rdfs:isDefinedBy rdf:datatype="http://www.w3.org/2001/XMLSchema#anyURI">https://developer.adobe.com/xmp/docs/XMPNamespaces/crs/</rdfs:isDefinedBy>
        <rdfs:label xml:lang="en">brightness</rdfs:label>
    </owl:Class>
    


    <!-- http://www.semanticweb.org/djebbia/ontologies/2022/8/untitled-ontology-22/cameraRawNamespace -->

    <owl:Class rdf:about="http://www.semanticweb.org/djebbia/ontologies/2022/8/untitled-ontology-22/cameraRawNamespace">
        <rdfs:subClassOf rdf:resource="http://www.semanticweb.org/djebbia/ontologies/2022/8/untitled-ontology-22/standards"/>
        <rdfs:comment xml:lang="en">CC BY-SA</rdfs:comment>
        <rdfs:comment xml:lang="en">The date and time the resource was last modified. NOTE: The value of this property is not necessarily the same as the file’s system modification date because it is typically set before the file is saved.</rdfs:comment>
        <rdfs:comment rdf:datatype="http://www.w3.org/2001/XMLSchema#anyURI">http://creativecommons.org/licenses/by-sa/4.0/</rdfs:comment>
        <rdfs:label xml:lang="en">cameraRawNamespace</rdfs:label>
    </owl:Class>
    


    <!-- http://www.semanticweb.org/djebbia/ontologies/2022/8/untitled-ontology-22/color_space -->

    <owl:Class rdf:about="http://www.semanticweb.org/djebbia/ontologies/2022/8/untitled-ontology-22/color_space">
        <rdfs:subClassOf rdf:resource="http://www.semanticweb.org/djebbia/ontologies/2022/8/untitled-ontology-22/multimedia_extended_metadata"/>
        <rdfs:comment xml:lang="en">CC BY-SA</rdfs:comment>
        <rdfs:comment xml:lang="en">EXIF tag 40961, 0xA001. Color space information:1 = sRGB, 65535 = uncalibrated</rdfs:comment>
        <rdfs:comment xml:lang="en">exif:ColorSpace</rdfs:comment>
        <rdfs:comment rdf:datatype="http://www.w3.org/2001/XMLSchema#anyURI">http://creativecommons.org/licenses/by-sa/4.0/</rdfs:comment>
        <rdfs:isDefinedBy rdf:datatype="http://www.w3.org/2001/XMLSchema#anyURI">https://developer.adobe.com/xmp/docs/XMPNamespaces/exif/</rdfs:isDefinedBy>
        <rdfs:label xml:lang="en">color_space</rdfs:label>
    </owl:Class>
    


    <!-- http://www.semanticweb.org/djebbia/ontologies/2022/8/untitled-ontology-22/contentType -->

    <owl:Class rdf:about="http://www.semanticweb.org/djebbia/ontologies/2022/8/untitled-ontology-22/contentType">
        <rdfs:subClassOf rdf:resource="http://www.semanticweb.org/djebbia/ontologies/2022/8/untitled-ontology-22/Multimedia"/>
        <rdfs:comment xml:lang="en">CC BY-SA</rdfs:comment>
        <rdfs:comment xml:lang="en">References the bioontology schema.</rdfs:comment>
        <rdfs:comment rdf:datatype="http://www.w3.org/2001/XMLSchema#anyURI">http://creativecommons.org/licenses/by-sa/4.0/</rdfs:comment>
        <rdfs:comment xml:lang="en">kindOfSpecimen </rdfs:comment>
        <rdfs:isDefinedBy rdf:datatype="http://www.w3.org/2001/XMLSchema#anyURI">https://bioportal.bioontology.org/ontologies/TDWGSPEC/?p=properties</rdfs:isDefinedBy>
        <rdfs:label xml:lang="en">contentType</rdfs:label>
    </owl:Class>
    


    <!-- http://www.semanticweb.org/djebbia/ontologies/2022/8/untitled-ontology-22/contrastProcessing -->

    <owl:Class rdf:about="http://www.semanticweb.org/djebbia/ontologies/2022/8/untitled-ontology-22/contrastProcessing">
        <rdfs:subClassOf rdf:resource="http://www.semanticweb.org/djebbia/ontologies/2022/8/untitled-ontology-22/multimedia_extended_metadata"/>
        <rdfs:comment xml:lang="en">CC BY-SA</rdfs:comment>
        <rdfs:comment xml:lang="en">Contrast setting. Range -50 to 100.</rdfs:comment>
        <rdfs:comment xml:lang="en">crs:Contrast</rdfs:comment>
        <rdfs:comment rdf:datatype="http://www.w3.org/2001/XMLSchema#anyURI">http://creativecommons.org/licenses/by-sa/4.0/</rdfs:comment>
        <rdfs:isDefinedBy rdf:datatype="http://www.w3.org/2001/XMLSchema#anyURI">https://developer.adobe.com/xmp/docs/XMPNamespaces/crs/</rdfs:isDefinedBy>
        <rdfs:label xml:lang="en">contrastProcessing</rdfs:label>
    </owl:Class>
    


    <!-- http://www.semanticweb.org/djebbia/ontologies/2022/8/untitled-ontology-22/contrastSetting -->

    <owl:Class rdf:about="http://www.semanticweb.org/djebbia/ontologies/2022/8/untitled-ontology-22/contrastSetting">
        <rdfs:subClassOf rdf:resource="http://www.semanticweb.org/djebbia/ontologies/2022/8/untitled-ontology-22/multimedia_extended_metadata"/>
        <rdfs:comment xml:lang="en">CC BY-SA</rdfs:comment>
        <rdfs:comment xml:lang="en">EXIF tag 41992, 0xA408. Indicates the direction of contrast processing applied by the camera:0 = Normal, 1 = Soft, 2 = Hard</rdfs:comment>
        <rdfs:comment xml:lang="en">exif:Contrast</rdfs:comment>
        <rdfs:comment rdf:datatype="http://www.w3.org/2001/XMLSchema#anyURI">http://creativecommons.org/licenses/by-sa/4.0/</rdfs:comment>
        <rdfs:isDefinedBy rdf:datatype="http://www.w3.org/2001/XMLSchema#anyURI">https://developer.adobe.com/xmp/docs/XMPNamespaces/exif/</rdfs:isDefinedBy>
        <rdfs:label xml:lang="en">contrastSetting</rdfs:label>
    </owl:Class>
    


    <!-- http://www.semanticweb.org/djebbia/ontologies/2022/8/untitled-ontology-22/createDateForImage -->

    <owl:Class rdf:about="http://www.semanticweb.org/djebbia/ontologies/2022/8/untitled-ontology-22/createDateForImage">
        <rdfs:subClassOf rdf:resource="http://www.semanticweb.org/djebbia/ontologies/2022/8/untitled-ontology-22/Multimedia"/>
        <rdfs:comment xml:lang="en">CC BY-SA</rdfs:comment>
        <rdfs:comment xml:lang="en">The creation date of the image. </rdfs:comment>
        <rdfs:comment rdf:datatype="http://www.w3.org/2001/XMLSchema#anyURI">http://creativecommons.org/licenses/by-sa/4.0/</rdfs:comment>
        <rdfs:comment xml:lang="en">xmp:CreateDate</rdfs:comment>
        <rdfs:isDefinedBy rdf:datatype="http://www.w3.org/2001/XMLSchema#anyURI">https://developer.adobe.com/xmp/docs/XMPNamespaces/xmp/</rdfs:isDefinedBy>
        <rdfs:label xml:lang="en">create date for image</rdfs:label>
    </owl:Class>
    


    <!-- http://www.semanticweb.org/djebbia/ontologies/2022/8/untitled-ontology-22/create_date -->

    <owl:Class rdf:about="http://www.semanticweb.org/djebbia/ontologies/2022/8/untitled-ontology-22/create_date">
        <rdfs:subClassOf rdf:resource="http://www.semanticweb.org/djebbia/ontologies/2022/8/untitled-ontology-22/IQ_metadata"/>
        <rdfs:subClassOf rdf:resource="http://www.semanticweb.org/djebbia/ontologies/2022/8/untitled-ontology-22/multimedia_extended_metadata"/>
        <rdfs:comment xml:lang="en">CC BY-SA</rdfs:comment>
        <rdfs:comment xml:lang="en">The creation date of the image. </rdfs:comment>
        <rdfs:comment xml:lang="en">The date and time the resource was created. For a digital file, this need not match a file-system creation time. For a freshly created resource, it should be close to that time, modulo the time taken to write the file. Later file transfer, copying, and so on, can make the file-system time arbitrarily different.</rdfs:comment>
        <rdfs:comment rdf:datatype="http://www.w3.org/2001/XMLSchema#anyURI">http://creativecommons.org/licenses/by-sa/4.0/</rdfs:comment>
        <rdfs:comment xml:lang="en">xmp:CreateDate</rdfs:comment>
        <rdfs:isDefinedBy rdf:datatype="http://www.w3.org/2001/XMLSchema#anyURI">https://developer.adobe.com/xmp/docs/XMPNamespaces/xmp/</rdfs:isDefinedBy>
        <rdfs:label xml:lang="en">create_date</rdfs:label>
    </owl:Class>
    


    <!-- http://www.semanticweb.org/djebbia/ontologies/2022/8/untitled-ontology-22/darwinCore -->

    <owl:Class rdf:about="http://www.semanticweb.org/djebbia/ontologies/2022/8/untitled-ontology-22/darwinCore">
        <rdfs:subClassOf rdf:resource="http://www.semanticweb.org/djebbia/ontologies/2022/8/untitled-ontology-22/standards"/>
        <rdfs:comment xml:lang="en">CC BY-SA</rdfs:comment>
        <rdfs:comment xml:lang="en">The date and time the resource was last modified. NOTE: The value of this property is not necessarily the same as the file’s system modification date because it is typically set before the file is saved.</rdfs:comment>
        <rdfs:comment rdf:datatype="http://www.w3.org/2001/XMLSchema#anyURI">http://creativecommons.org/licenses/by-sa/4.0/</rdfs:comment>
        <rdfs:label xml:lang="en">darwinCore</rdfs:label>
    </owl:Class>
    


    <!-- http://www.semanticweb.org/djebbia/ontologies/2022/8/untitled-ontology-22/data_capture_method -->

    <owl:Class rdf:about="http://www.semanticweb.org/djebbia/ontologies/2022/8/untitled-ontology-22/data_capture_method">
        <rdfs:subClassOf rdf:resource="http://www.semanticweb.org/djebbia/ontologies/2022/8/untitled-ontology-22/Multimedia"/>
        <rdfs:comment xml:lang="en">CC BY-SA</rdfs:comment>
        <rdfs:comment xml:lang="en">Information about technical aspects of the creation and digitization process of the resource. This includes modification steps (&quot;retouching&quot;) after the initial resource capture.</rdfs:comment>
        <rdfs:comment xml:lang="en">ac:resourceCreationTechnique</rdfs:comment>
        <rdfs:comment rdf:datatype="http://www.w3.org/2001/XMLSchema#anyURI">http://creativecommons.org/licenses/by-sa/4.0/</rdfs:comment>
        <rdfs:isDefinedBy rdf:datatype="http://www.w3.org/2001/XMLSchema#anyURI">http://rs.tdwg.org/ac/terms/resourceCreationTechnique</rdfs:isDefinedBy>
        <rdfs:label xml:lang="en">data_capture_method</rdfs:label>
    </owl:Class>
    


    <!-- http://www.semanticweb.org/djebbia/ontologies/2022/8/untitled-ontology-22/dublinCore -->

    <owl:Class rdf:about="http://www.semanticweb.org/djebbia/ontologies/2022/8/untitled-ontology-22/dublinCore">
        <rdfs:subClassOf rdf:resource="http://www.semanticweb.org/djebbia/ontologies/2022/8/untitled-ontology-22/standards"/>
        <rdfs:comment xml:lang="en">CC BY-SA</rdfs:comment>
        <rdfs:comment xml:lang="en">The date and time the resource was last modified. NOTE: The value of this property is not necessarily the same as the file’s system modification date because it is typically set before the file is saved.</rdfs:comment>
        <rdfs:comment rdf:datatype="http://www.w3.org/2001/XMLSchema#anyURI">http://creativecommons.org/licenses/by-sa/4.0/</rdfs:comment>
        <rdfs:label xml:lang="en">dublinCore</rdfs:label>
    </owl:Class>
    


    <!-- http://www.semanticweb.org/djebbia/ontologies/2022/8/untitled-ontology-22/exposure -->

    <owl:Class rdf:about="http://www.semanticweb.org/djebbia/ontologies/2022/8/untitled-ontology-22/exposure">
        <rdfs:subClassOf rdf:resource="http://www.semanticweb.org/djebbia/ontologies/2022/8/untitled-ontology-22/multimedia_extended_metadata"/>
        <rdfs:comment xml:lang="en">CC BY-SA</rdfs:comment>
        <rdfs:comment xml:lang="en">Exposure setting. Range -4.0 to 4.0.</rdfs:comment>
        <rdfs:comment xml:lang="en">crs:Exposure</rdfs:comment>
        <rdfs:comment rdf:datatype="http://www.w3.org/2001/XMLSchema#anyURI">http://creativecommons.org/licenses/by-sa/4.0/</rdfs:comment>
        <rdfs:isDefinedBy rdf:datatype="http://www.w3.org/2001/XMLSchema#anyURI">https://developer.adobe.com/xmp/docs/XMPNamespaces/crs/</rdfs:isDefinedBy>
        <rdfs:label xml:lang="en">exposure</rdfs:label>
    </owl:Class>
    


    <!-- http://www.semanticweb.org/djebbia/ontologies/2022/8/untitled-ontology-22/file_extention -->

    <owl:Class rdf:about="http://www.semanticweb.org/djebbia/ontologies/2022/8/untitled-ontology-22/file_extention">
        <rdfs:subClassOf rdf:resource="http://www.semanticweb.org/djebbia/ontologies/2022/8/untitled-ontology-22/Multimedia"/>
        <rdfs:subClassOf rdf:resource="http://www.semanticweb.org/djebbia/ontologies/2022/8/untitled-ontology-22/multimedia_extended_metadata"/>
        <rdfs:comment xml:lang="en">CC BY-SA</rdfs:comment>
        <rdfs:comment xml:lang="en">The file format, physical medium, or dimensions of the resource.</rdfs:comment>
        <rdfs:comment xml:lang="en">dc:format</rdfs:comment>
        <rdfs:comment xml:lang="en">he file format, physical medium, or dimensions of the resource.Recommended practice is to use a controlled vocabulary where available. For example, for file formats one could use the list of Internet Media Types [MIME].</rdfs:comment>
        <rdfs:comment rdf:datatype="http://www.w3.org/2001/XMLSchema#anyURI">http://creativecommons.org/licenses/by-sa/4.0/</rdfs:comment>
        <rdfs:isDefinedBy rdf:datatype="http://www.w3.org/2001/XMLSchema#anyURI">http://purl.org/dc/elements/1.1/format</rdfs:isDefinedBy>
        <rdfs:label xml:lang="en">file_extention</rdfs:label>
    </owl:Class>
    


    <!-- http://www.semanticweb.org/djebbia/ontologies/2022/8/untitled-ontology-22/height -->

    <owl:Class rdf:about="http://www.semanticweb.org/djebbia/ontologies/2022/8/untitled-ontology-22/height">
        <rdfs:subClassOf rdf:resource="http://www.semanticweb.org/djebbia/ontologies/2022/8/untitled-ontology-22/multimedia_extended_metadata"/>
        <rdfs:comment xml:lang="en">CC BY-SA</rdfs:comment>
        <rdfs:comment xml:lang="en">EXIF tag 40963, 0xA003. Valid image height, in pixels.</rdfs:comment>
        <rdfs:comment xml:lang="en">exif:PixelYDimension</rdfs:comment>
        <rdfs:comment rdf:datatype="http://www.w3.org/2001/XMLSchema#anyURI">http://creativecommons.org/licenses/by-sa/4.0/</rdfs:comment>
        <rdfs:isDefinedBy rdf:datatype="http://www.w3.org/2001/XMLSchema#anyURI">http://ns.adobe.com/exif/1.0/PixelXDimension</rdfs:isDefinedBy>
        <rdfs:label xml:lang="en">height</rdfs:label>
    </owl:Class>
    


    <!-- http://www.semanticweb.org/djebbia/ontologies/2022/8/untitled-ontology-22/language -->

    <owl:Class rdf:about="http://www.semanticweb.org/djebbia/ontologies/2022/8/untitled-ontology-22/language">
        <rdfs:subClassOf rdf:resource="http://www.semanticweb.org/djebbia/ontologies/2022/8/untitled-ontology-22/Multimedia"/>
        <rdfs:comment xml:lang="en">CC BY-SA</rdfs:comment>
        <rdfs:comment xml:lang="en">The language of the resource. </rdfs:comment>
        <rdfs:comment xml:lang="en">dc:language</rdfs:comment>
        <rdfs:comment rdf:datatype="http://www.w3.org/2001/XMLSchema#anyURI">http://creativecommons.org/licenses/by-sa/4.0/</rdfs:comment>
        <rdfs:isDefinedBy rdf:datatype="http://www.w3.org/2001/XMLSchema#anyURI">http://purl.org/dc/terms/language</rdfs:isDefinedBy>
        <rdfs:label xml:lang="en">language</rdfs:label>
    </owl:Class>
    


    <!-- http://www.semanticweb.org/djebbia/ontologies/2022/8/untitled-ontology-22/license -->

    <owl:Class rdf:about="http://www.semanticweb.org/djebbia/ontologies/2022/8/untitled-ontology-22/license">
        <rdfs:subClassOf rdf:resource="http://www.semanticweb.org/djebbia/ontologies/2022/8/untitled-ontology-22/IQ_metadata"/>
        <rdfs:subClassOf rdf:resource="http://www.semanticweb.org/djebbia/ontologies/2022/8/untitled-ontology-22/Multimedia"/>
        <rdfs:subClassOf rdf:resource="http://www.semanticweb.org/djebbia/ontologies/2022/8/untitled-ontology-22/multimedia_extended_metadata"/>
        <rdfs:comment xml:lang="en">CC BY-SA</rdfs:comment>
        <rdfs:comment xml:lang="en">URL</rdfs:comment>
        <rdfs:comment xml:lang="en">dc:license</rdfs:comment>
        <rdfs:comment xml:lang="en">dwc:license</rdfs:comment>
        <rdfs:comment xml:lang="en">http://creativecommons.org/licenses/by-sa/4.0/</rdfs:comment>
        <rdfs:comment rdf:datatype="http://www.w3.org/2001/XMLSchema#anyURI">http://creativecommons.org/licenses/by-sa/4.0/</rdfs:comment>
        <rdfs:comment xml:lang="en">http://creativecommons.org/licenses/by/4.0/</rdfs:comment>
        <rdfs:isDefinedBy rdf:datatype="http://www.w3.org/2001/XMLSchema#anyURI">http://purl.org/dc/terms/license</rdfs:isDefinedBy>
        <rdfs:label xml:lang="en">license</rdfs:label>
    </owl:Class>
    


    <!-- http://www.semanticweb.org/djebbia/ontologies/2022/8/untitled-ontology-22/measurementType -->

    <owl:Class rdf:about="http://www.semanticweb.org/djebbia/ontologies/2022/8/untitled-ontology-22/measurementType">
        <rdfs:subClassOf rdf:resource="http://www.semanticweb.org/djebbia/ontologies/2022/8/untitled-ontology-22/multimedia_extended_metadata"/>
        <rdfs:comment xml:lang="en">CC BY-SA</rdfs:comment>
        <rdfs:comment xml:lang="en">The nature of the measurement, fact, characteristic, or assertion.</rdfs:comment>
        <rdfs:comment xml:lang="en">dwc:measurementType</rdfs:comment>
        <rdfs:comment rdf:datatype="http://www.w3.org/2001/XMLSchema#anyURI">http://creativecommons.org/licenses/by-sa/4.0/</rdfs:comment>
        <rdfs:isDefinedBy rdf:datatype="http://www.w3.org/2001/XMLSchema#anyURI">http://rs.tdwg.org/dwc/iri/measurementType</rdfs:isDefinedBy>
        <rdfs:label xml:lang="en">measurementType</rdfs:label>
    </owl:Class>
    


    <!-- http://www.semanticweb.org/djebbia/ontologies/2022/8/untitled-ontology-22/measurementUnit -->

    <owl:Class rdf:about="http://www.semanticweb.org/djebbia/ontologies/2022/8/untitled-ontology-22/measurementUnit">
        <rdfs:subClassOf rdf:resource="http://www.semanticweb.org/djebbia/ontologies/2022/8/untitled-ontology-22/multimedia_extended_metadata"/>
        <rdfs:comment xml:lang="en">CC BY-SA</rdfs:comment>
        <rdfs:comment xml:lang="en">The units associated with the measurementValue.</rdfs:comment>
        <rdfs:comment xml:lang="en">dwc:measurementUnit</rdfs:comment>
        <rdfs:comment rdf:datatype="http://www.w3.org/2001/XMLSchema#anyURI">http://creativecommons.org/licenses/by-sa/4.0/</rdfs:comment>
        <rdfs:isDefinedBy rdf:datatype="http://www.w3.org/2001/XMLSchema#anyURI">http://rs.tdwg.org/dwc/iri/measurementUnit</rdfs:isDefinedBy>
        <rdfs:label xml:lang="en">measurementUnit</rdfs:label>
    </owl:Class>
    


    <!-- http://www.semanticweb.org/djebbia/ontologies/2022/8/untitled-ontology-22/modifyDateForImage -->

    <owl:Class rdf:about="http://www.semanticweb.org/djebbia/ontologies/2022/8/untitled-ontology-22/modifyDateForImage">
        <rdfs:subClassOf rdf:resource="http://www.semanticweb.org/djebbia/ontologies/2022/8/untitled-ontology-22/Multimedia"/>
        <rdfs:comment xml:lang="en">CC BY-SA</rdfs:comment>
        <rdfs:comment xml:lang="en">The date and time that any metadata for this resource was last changed. It should be the same as or more recent than xmp:ModifyDate.</rdfs:comment>
        <rdfs:comment rdf:datatype="http://www.w3.org/2001/XMLSchema#anyURI">http://creativecommons.org/licenses/by-sa/4.0/</rdfs:comment>
        <rdfs:comment xml:lang="en">xmp:ModifyDate</rdfs:comment>
        <rdfs:isDefinedBy rdf:datatype="http://www.w3.org/2001/XMLSchema#anyURI">https://developer.adobe.com/xmp/docs/XMPNamespaces/xmp/</rdfs:isDefinedBy>
        <rdfs:label xml:lang="en">modify date for image</rdfs:label>
    </owl:Class>
    


    <!-- http://www.semanticweb.org/djebbia/ontologies/2022/8/untitled-ontology-22/modifyDateForImageMetadata -->

    <owl:Class rdf:about="http://www.semanticweb.org/djebbia/ontologies/2022/8/untitled-ontology-22/modifyDateForImageMetadata">
        <rdfs:subClassOf rdf:resource="http://www.semanticweb.org/djebbia/ontologies/2022/8/untitled-ontology-22/Multimedia"/>
        <rdfs:comment xml:lang="en">CC BY-SA</rdfs:comment>
        <rdfs:comment xml:lang="en">The date and time the resource was last modified. NOTE: The value of this property is not necessarily the same as the file’s system modification date because it is typically set before the file is saved.</rdfs:comment>
        <rdfs:comment rdf:datatype="http://www.w3.org/2001/XMLSchema#anyURI">http://creativecommons.org/licenses/by-sa/4.0/</rdfs:comment>
        <rdfs:comment xml:lang="en">xmp:MetadataDate</rdfs:comment>
        <rdfs:isDefinedBy rdf:datatype="http://www.w3.org/2001/XMLSchema#anyURI">https://developer.adobe.com/xmp/docs/XMPNamespaces/xmp/</rdfs:isDefinedBy>
        <rdfs:label xml:lang="en">modify date for image metadata</rdfs:label>
    </owl:Class>
    


    <!-- http://www.semanticweb.org/djebbia/ontologies/2022/8/untitled-ontology-22/multimedia_extended_metadata -->

    <owl:Class rdf:about="http://www.semanticweb.org/djebbia/ontologies/2022/8/untitled-ontology-22/multimedia_extended_metadata"/>
    


    <!-- http://www.semanticweb.org/djebbia/ontologies/2022/8/untitled-ontology-22/organismQuantityType -->

    <owl:Class rdf:about="http://www.semanticweb.org/djebbia/ontologies/2022/8/untitled-ontology-22/organismQuantityType">
        <rdfs:subClassOf rdf:resource="http://www.semanticweb.org/djebbia/ontologies/2022/8/untitled-ontology-22/multimedia_extended_metadata"/>
        <rdfs:comment xml:lang="en">CC BY-SA</rdfs:comment>
        <rdfs:comment xml:lang="en">The type of quantification system used for the quantity of organisms. In the case of TUBRI dwc:individuals</rdfs:comment>
        <rdfs:comment xml:lang="en">dwc:organismQuantityType</rdfs:comment>
        <rdfs:comment rdf:datatype="http://www.w3.org/2001/XMLSchema#anyURI">http://creativecommons.org/licenses/by-sa/4.0/</rdfs:comment>
        <rdfs:isDefinedBy rdf:datatype="http://www.w3.org/2001/XMLSchema#anyURI">http://rs.tdwg.org/dwc/terms/organismQuantityType</rdfs:isDefinedBy>
        <rdfs:label xml:lang="en">organismQuantityType</rdfs:label>
    </owl:Class>
    


    <!-- http://www.semanticweb.org/djebbia/ontologies/2022/8/untitled-ontology-22/original_filename -->

    <owl:Class rdf:about="http://www.semanticweb.org/djebbia/ontologies/2022/8/untitled-ontology-22/original_filename">
        <rdfs:subClassOf rdf:resource="http://www.semanticweb.org/djebbia/ontologies/2022/8/untitled-ontology-22/Multimedia"/>
        <rdfs:subClassOf rdf:resource="http://www.semanticweb.org/djebbia/ontologies/2022/8/untitled-ontology-22/multimedia_extended_metadata"/>
        <rdfs:comment xml:lang="en">CC BY-SA</rdfs:comment>
        <rdfs:comment rdf:datatype="http://www.w3.org/2001/XMLSchema#anyURI">http://creativecommons.org/licenses/by-sa/4.0/</rdfs:comment>
        <rdfs:comment xml:lang="en">plus:FileNameAsDelivered</rdfs:comment>
        <rdfs:isDefinedBy rdf:datatype="http://www.w3.org/2001/XMLSchema#anyURI">https://developer.adobe.com/xmp/docs/XMPNamespaces/xmp/</rdfs:isDefinedBy>
        <rdfs:label xml:lang="en">original_filename</rdfs:label>
    </owl:Class>
    


    <!-- http://www.semanticweb.org/djebbia/ontologies/2022/8/untitled-ontology-22/ownership -->

    <owl:Class rdf:about="http://www.semanticweb.org/djebbia/ontologies/2022/8/untitled-ontology-22/ownership">
        <rdfs:subClassOf rdf:resource="http://www.semanticweb.org/djebbia/ontologies/2022/8/untitled-ontology-22/IQ_metadata"/>
        <rdfs:subClassOf rdf:resource="http://www.semanticweb.org/djebbia/ontologies/2022/8/untitled-ontology-22/Multimedia"/>
        <rdfs:subClassOf rdf:resource="http://www.semanticweb.org/djebbia/ontologies/2022/8/untitled-ontology-22/multimedia_extended_metadata"/>
        <rdfs:comment xml:lang="en">CC BY-SA</rdfs:comment>
        <rdfs:comment xml:lang="en">The name (or acronym) in use by the institution having ownership of the object(s) or information referred to in the record.</rdfs:comment>
        <rdfs:comment xml:lang="en">dwc:ownerInstitutionCode</rdfs:comment>
        <rdfs:comment rdf:datatype="http://www.w3.org/2001/XMLSchema#anyURI">http://creativecommons.org/licenses/by-sa/4.0/</rdfs:comment>
        <rdfs:isDefinedBy rdf:datatype="http://www.w3.org/2001/XMLSchema#anyURI">http://rs.tdwg.org/dwc/terms/ownerInstitutionCode</rdfs:isDefinedBy>
        <rdfs:label xml:lang="en">ownership</rdfs:label>
    </owl:Class>
    


    <!-- http://www.semanticweb.org/djebbia/ontologies/2022/8/untitled-ontology-22/parent_arc_id -->

    <owl:Class rdf:about="http://www.semanticweb.org/djebbia/ontologies/2022/8/untitled-ontology-22/parent_arc_id">
        <rdfs:subClassOf rdf:resource="http://www.semanticweb.org/djebbia/ontologies/2022/8/untitled-ontology-22/Multimedia"/>
        <rdfs:comment xml:lang="en">CC BY-SA</rdfs:comment>
        <rdfs:comment xml:lang="en">dwc:associatedMedia</rdfs:comment>
        <rdfs:comment rdf:datatype="http://www.w3.org/2001/XMLSchema#anyURI">http://creativecommons.org/licenses/by-sa/4.0/</rdfs:comment>
        <rdfs:isDefinedBy rdf:datatype="http://www.w3.org/2001/XMLSchema#anyURI">A list (concatenated and separated) of identifiers (publication, global unique identifier, URI) of media associated with the Occurrence.</rdfs:isDefinedBy>
        <rdfs:label xml:lang="en">parent_arc_id</rdfs:label>
    </owl:Class>
    


    <!-- http://www.semanticweb.org/djebbia/ontologies/2022/8/untitled-ontology-22/path -->

    <owl:Class rdf:about="http://www.semanticweb.org/djebbia/ontologies/2022/8/untitled-ontology-22/path">
        <rdfs:subClassOf rdf:resource="http://www.semanticweb.org/djebbia/ontologies/2022/8/untitled-ontology-22/Multimedia"/>
        <rdfs:comment xml:lang="en">CC BY-SA</rdfs:comment>
        <rdfs:comment xml:lang="en">ac:accessURI</rdfs:comment>
        <rdfs:comment rdf:datatype="http://www.w3.org/2001/XMLSchema#anyURI">http://creativecommons.org/licenses/by-sa/4.0/</rdfs:comment>
        <rdfs:comment xml:lang="en">https://bgnn.tulane.edu/</rdfs:comment>
        <rdfs:isDefinedBy rdf:datatype="http://www.w3.org/2001/XMLSchema#anyURI">http://rs.tdwg.org/ac/terms/accessURI</rdfs:isDefinedBy>
        <rdfs:label xml:lang="en">path</rdfs:label>
    </owl:Class>
    


    <!-- http://www.semanticweb.org/djebbia/ontologies/2022/8/untitled-ontology-22/publisher -->

    <owl:Class rdf:about="http://www.semanticweb.org/djebbia/ontologies/2022/8/untitled-ontology-22/publisher">
        <rdfs:subClassOf rdf:resource="http://www.semanticweb.org/djebbia/ontologies/2022/8/untitled-ontology-22/Multimedia"/>
        <rdfs:comment xml:lang="en">CC BY-SA</rdfs:comment>
        <rdfs:comment xml:lang="en">Tulane University Biodiversity Research Institute</rdfs:comment>
        <rdfs:comment xml:lang="en">dc:publisher</rdfs:comment>
        <rdfs:comment rdf:datatype="http://www.w3.org/2001/XMLSchema#anyURI">http://creativecommons.org/licenses/by-sa/4.0/</rdfs:comment>
        <rdfs:isDefinedBy rdf:datatype="http://www.w3.org/2001/XMLSchema#anyURI">http://purl.org/dc/terms/publisher</rdfs:isDefinedBy>
        <rdfs:label xml:lang="en">publisher</rdfs:label>
    </owl:Class>
    


    <!-- http://www.semanticweb.org/djebbia/ontologies/2022/8/untitled-ontology-22/resourceCreationTechnique -->

    <owl:Class rdf:about="http://www.semanticweb.org/djebbia/ontologies/2022/8/untitled-ontology-22/resourceCreationTechnique">
        <rdfs:subClassOf rdf:resource="http://www.semanticweb.org/djebbia/ontologies/2022/8/untitled-ontology-22/multimedia_extended_metadata"/>
        <rdfs:comment xml:lang="en">CC BY-SA</rdfs:comment>
        <rdfs:comment xml:lang="en">Information about technical aspects of the creation and digitization process of the resource. This includes modification steps (&quot;retouching&quot;) after the initial resource capture.</rdfs:comment>
        <rdfs:comment xml:lang="en">ac:resourceCreationTechnique</rdfs:comment>
        <rdfs:comment rdf:datatype="http://www.w3.org/2001/XMLSchema#anyURI">http://creativecommons.org/licenses/by-sa/4.0/</rdfs:comment>
        <rdfs:isDefinedBy rdf:datatype="http://www.w3.org/2001/XMLSchema#anyURI">http://rs.tdwg.org/ac/terms/resourceCreationTechnique</rdfs:isDefinedBy>
        <rdfs:label xml:lang="en">resourceCreationTechnique</rdfs:label>
    </owl:Class>
    


    <!-- http://www.semanticweb.org/djebbia/ontologies/2022/8/untitled-ontology-22/rightsHolder -->

    <owl:Class rdf:about="http://www.semanticweb.org/djebbia/ontologies/2022/8/untitled-ontology-22/rightsHolder">
        <rdfs:subClassOf rdf:resource="http://www.semanticweb.org/djebbia/ontologies/2022/8/untitled-ontology-22/Multimedia"/>
        <rdfs:comment xml:lang="en">A person or organization owning or managing rights over the resource.</rdfs:comment>
        <rdfs:comment xml:lang="en">CC BY-SA</rdfs:comment>
        <rdfs:comment xml:lang="en">dc:rightsHolder</rdfs:comment>
        <rdfs:comment rdf:datatype="http://www.w3.org/2001/XMLSchema#anyURI">http://creativecommons.org/licenses/by-sa/4.0/</rdfs:comment>
        <rdfs:isDefinedBy rdf:datatype="http://www.w3.org/2001/XMLSchema#anyURI">http://purl.org/dc/terms/rightsHolder</rdfs:isDefinedBy>
        <rdfs:label xml:lang="en">rightsHolder</rdfs:label>
    </owl:Class>
    


    <!-- http://www.semanticweb.org/djebbia/ontologies/2022/8/untitled-ontology-22/saturation -->

    <owl:Class rdf:about="http://www.semanticweb.org/djebbia/ontologies/2022/8/untitled-ontology-22/saturation">
        <rdfs:subClassOf rdf:resource="http://www.semanticweb.org/djebbia/ontologies/2022/8/untitled-ontology-22/multimedia_extended_metadata"/>
        <rdfs:comment xml:lang="en">CC BY-SA</rdfs:comment>
        <rdfs:comment xml:lang="en">Saturation setting. Range -100 to 100.</rdfs:comment>
        <rdfs:comment xml:lang="en">crs:Saturation</rdfs:comment>
        <rdfs:comment rdf:datatype="http://www.w3.org/2001/XMLSchema#anyURI">http://creativecommons.org/licenses/by-sa/4.0/</rdfs:comment>
        <rdfs:isDefinedBy rdf:datatype="http://www.w3.org/2001/XMLSchema#anyURI">https://developer.adobe.com/xmp/docs/XMPNamespaces/crs/</rdfs:isDefinedBy>
        <rdfs:label xml:lang="en">saturation</rdfs:label>
    </owl:Class>
    


    <!-- http://www.semanticweb.org/djebbia/ontologies/2022/8/untitled-ontology-22/saturationProcessing -->

    <owl:Class rdf:about="http://www.semanticweb.org/djebbia/ontologies/2022/8/untitled-ontology-22/saturationProcessing">
        <rdfs:subClassOf rdf:resource="http://www.semanticweb.org/djebbia/ontologies/2022/8/untitled-ontology-22/multimedia_extended_metadata"/>
        <rdfs:comment xml:lang="en">CC BY-SA</rdfs:comment>
        <rdfs:comment xml:lang="en">EXIF tag 41993, 0xA409. Indicates the direction of saturation processing applied by the camera: 0 = Normal, 1 = Low saturation, 2 = High saturation</rdfs:comment>
        <rdfs:comment xml:lang="en">exif:Saturation</rdfs:comment>
        <rdfs:comment rdf:datatype="http://www.w3.org/2001/XMLSchema#anyURI">http://creativecommons.org/licenses/by-sa/4.0/</rdfs:comment>
        <rdfs:isDefinedBy rdf:datatype="http://www.w3.org/2001/XMLSchema#anyURI">https://developer.adobe.com/xmp/docs/XMPNamespaces/exif/</rdfs:isDefinedBy>
        <rdfs:label xml:lang="en">saturationProcessing</rdfs:label>
    </owl:Class>
    


    <!-- http://www.semanticweb.org/djebbia/ontologies/2022/8/untitled-ontology-22/size -->

    <owl:Class rdf:about="http://www.semanticweb.org/djebbia/ontologies/2022/8/untitled-ontology-22/size">
        <rdfs:subClassOf rdf:resource="http://www.semanticweb.org/djebbia/ontologies/2022/8/untitled-ontology-22/multimedia_extended_metadata"/>
        <rdfs:comment xml:lang="en">CC BY-SA</rdfs:comment>
        <rdfs:comment xml:lang="en">The size or duration of the resource. Recommended practice is to specify the file size in megabytes and duration in ISO 8601 format.</rdfs:comment>
        <rdfs:comment xml:lang="en">dc:extent</rdfs:comment>
        <rdfs:comment rdf:datatype="http://www.w3.org/2001/XMLSchema#anyURI">http://creativecommons.org/licenses/by-sa/4.0/</rdfs:comment>
        <rdfs:isDefinedBy rdf:datatype="http://www.w3.org/2001/XMLSchema#anyURI">http://purl.org/dc/terms/extent</rdfs:isDefinedBy>
        <rdfs:label xml:lang="en">size</rdfs:label>
    </owl:Class>
    


    <!-- http://www.semanticweb.org/djebbia/ontologies/2022/8/untitled-ontology-22/source -->

    <owl:Class rdf:about="http://www.semanticweb.org/djebbia/ontologies/2022/8/untitled-ontology-22/source">
        <rdfs:subClassOf rdf:resource="http://www.semanticweb.org/djebbia/ontologies/2022/8/untitled-ontology-22/IQ_metadata"/>
        <rdfs:subClassOf rdf:resource="http://www.semanticweb.org/djebbia/ontologies/2022/8/untitled-ontology-22/Multimedia"/>
        <rdfs:subClassOf rdf:resource="http://www.semanticweb.org/djebbia/ontologies/2022/8/untitled-ontology-22/multimedia_extended_metadata"/>
        <rdfs:comment xml:lang="en">An entity responsible for making the resource available.</rdfs:comment>
        <rdfs:comment xml:lang="en">CC BY-SA</rdfs:comment>
        <rdfs:comment xml:lang="en">Source.</rdfs:comment>
        <rdfs:comment xml:lang="en">Tulane University Biodiversity Research Institute </rdfs:comment>
        <rdfs:comment xml:lang="en">dc:publisher</rdfs:comment>
        <rdfs:comment rdf:datatype="http://www.w3.org/2001/XMLSchema#anyURI">http://creativecommons.org/licenses/by-sa/4.0/</rdfs:comment>
        <rdfs:comment xml:lang="en">photoshop:Source</rdfs:comment>
        <rdfs:isDefinedBy rdf:datatype="http://www.w3.org/2001/XMLSchema#anyURI">developer.adobe.com/xmp/docs/XMPNamespaces/photoshop/</rdfs:isDefinedBy>
        <rdfs:isDefinedBy rdf:datatype="http://www.w3.org/2001/XMLSchema#anyURI">http://purl.org/dc/terms/publisher</rdfs:isDefinedBy>
        <rdfs:label xml:lang="en">source</rdfs:label>
    </owl:Class>
    


    <!-- http://www.semanticweb.org/djebbia/ontologies/2022/8/untitled-ontology-22/standards -->

    <owl:Class rdf:about="http://www.semanticweb.org/djebbia/ontologies/2022/8/untitled-ontology-22/standards"/>
    


    <!-- http://www.semanticweb.org/djebbia/ontologies/2022/8/untitled-ontology-22/type -->

    <owl:Class rdf:about="http://www.semanticweb.org/djebbia/ontologies/2022/8/untitled-ontology-22/type">
        <rdfs:subClassOf rdf:resource="http://www.semanticweb.org/djebbia/ontologies/2022/8/untitled-ontology-22/Multimedia"/>
        <rdfs:comment xml:lang="en">CC BY-SA</rdfs:comment>
        <rdfs:comment xml:lang="en">The nature or genre of the resource.</rdfs:comment>
        <rdfs:comment xml:lang="en">dc:type</rdfs:comment>
        <rdfs:comment rdf:datatype="http://www.w3.org/2001/XMLSchema#anyURI">http://creativecommons.org/licenses/by-sa/4.0/</rdfs:comment>
        <rdfs:isDefinedBy rdf:datatype="http://www.w3.org/2001/XMLSchema#anyURI">http://purl.org/dc/elements/1.1/type</rdfs:isDefinedBy>
        <rdfs:label xml:lang="en">type</rdfs:label>
    </owl:Class>
    


    <!-- http://www.semanticweb.org/djebbia/ontologies/2022/8/untitled-ontology-22/update_date -->

    <owl:Class rdf:about="http://www.semanticweb.org/djebbia/ontologies/2022/8/untitled-ontology-22/update_date">
        <rdfs:subClassOf rdf:resource="http://www.semanticweb.org/djebbia/ontologies/2022/8/untitled-ontology-22/multimedia_extended_metadata"/>
        <rdfs:comment xml:lang="en">CC BY-SA</rdfs:comment>
        <rdfs:comment xml:lang="en">The date and time the resource was last modified. NOTE: The value of this property is not necessarily the same as the file’s system modification date because it is typically set before the file is saved.</rdfs:comment>
        <rdfs:comment rdf:datatype="http://www.w3.org/2001/XMLSchema#anyURI">http://creativecommons.org/licenses/by-sa/4.0/</rdfs:comment>
        <rdfs:comment xml:lang="en">xmp:MetadataDate</rdfs:comment>
        <rdfs:isDefinedBy rdf:datatype="http://www.w3.org/2001/XMLSchema#anyURI">https://developer.adobe.com/xmp/docs/XMPNamespaces/xmp/</rdfs:isDefinedBy>
        <rdfs:label xml:lang="en">update_date</rdfs:label>
    </owl:Class>
    


    <!-- http://www.semanticweb.org/djebbia/ontologies/2022/8/untitled-ontology-22/width -->

    <owl:Class rdf:about="http://www.semanticweb.org/djebbia/ontologies/2022/8/untitled-ontology-22/width">
        <rdfs:subClassOf rdf:resource="http://www.semanticweb.org/djebbia/ontologies/2022/8/untitled-ontology-22/multimedia_extended_metadata"/>
        <rdfs:comment xml:lang="en">CC BY-SA</rdfs:comment>
        <rdfs:comment xml:lang="en">EXIF tag 40962, 0xA002. Valid image width, in pixels.</rdfs:comment>
        <rdfs:comment xml:lang="en">exif:PixelXDimension</rdfs:comment>
        <rdfs:comment rdf:datatype="http://www.w3.org/2001/XMLSchema#anyURI">http://creativecommons.org/licenses/by-sa/4.0/</rdfs:comment>
        <rdfs:isDefinedBy rdf:datatype="http://www.w3.org/2001/XMLSchema#anyURI">http://ns.adobe.com/exif/1.0/PixelYDimension</rdfs:isDefinedBy>
        <rdfs:label xml:lang="en">width</rdfs:label>
    </owl:Class>
    


    <!-- 
    ///////////////////////////////////////////////////////////////////////////////////////
    //
    // General axioms
    //
    ///////////////////////////////////////////////////////////////////////////////////////
     -->

    <rdf:Description>
        <rdf:type rdf:resource="http://www.w3.org/2002/07/owl#AllDisjointClasses"/>
        <owl:members rdf:parseType="Collection">
            <rdf:Description rdf:about="http://www.semanticweb.org/djebbia/ontologies/2022/8/untitled-ontology-22/IQ_metadata"/>
            <rdf:Description rdf:about="http://www.semanticweb.org/djebbia/ontologies/2022/8/untitled-ontology-22/Multimedia"/>
            <rdf:Description rdf:about="http://www.semanticweb.org/djebbia/ontologies/2022/8/untitled-ontology-22/multimedia_extended_metadata"/>
            <rdf:Description rdf:about="http://www.semanticweb.org/djebbia/ontologies/2022/8/untitled-ontology-22/standards"/>
        </owl:members>
    </rdf:Description>
</rdf:RDF>



<!-- Generated by the OWL API (version 4.5.9.2019-02-01T07:24:44Z) https://github.com/owlcs/owlapi -->

